# Number sequence

## Procedure

+ Given \\( a_{n+1} = k a_n + p a_{n-1} \\), \\( a_{n+1} - x a_n = (k - x) (a_n - x a_{n-1}) \\) where \\( x^2 = k x + p \\)

## Procedure: `y = x` Model

[Baidu Scholar](https://web.archive.org/web/20210111115001/https://xueshu.baidu.com/usercenter/paper/show?paperid=1k6y0j30tp4t0pb0gp1k0e30mv292076&site=xueshu_se)
[ixueshu](https://web.archive.org/web/20210111115140/https://www.ixueshu.com/document/e593e93b446046f386b00900c86b1678318947a18e7f9386.html)

### NCEE

数列 { \\( a_n \\) } 满足 \\( a_1 = a \\)， \\( a_{n+1} = a_n^2 + a \\) 且 \\( \left\lvert a_n \right\rvert \leq 2 \\)， 则 \\( a \\) 的取值范围为 （）

A. \[-2,2\] B. \[-2,0\] C. \[0,\\( \frac{1}{4} \\)\] D. \[-2,\\( \frac{1}{4}\\)\]

## Scaling

[Wikipedia](https://web.archive.org/web/20210120124018/https://zh.wikipedia.org/wiki/%E6%94%BE%E7%BC%A9%E6%B3%95)

\\(a_1\frac{1-q^n}{1-q}\leq\frac{a_1}{1-q}\\) where \\(q\in\(0,1\)\\)
